case_studies/atomic_test/output/atomic_test/proofs/proof_test_usize_cas_weak.v
@@ -1,0 +1,22 @@
+From caesium Require Import lang notation.
+From refinedrust Require Import typing shims.
+From refinedrust.examples.atomic_test.generated Require Import generated_code_atomic_test generated_specs_atomic_test generated_template_test_usize_cas_weak.
+
+Set Default Proof Using "Type".
+
+Section proof.
+Context `{RRGS : !refinedrustGS Σ}.
+
+Lemma test_usize_cas_weak_proof (π : thread_id) :
+  test_usize_cas_weak_lemma π.
+Proof.
+  test_usize_cas_weak_prelude.
+
+  rep <-! liRStep; liShow.
+
+  all: print_remaining_goal.
+  Unshelve. all: sidecond_solver.
+  Unshelve. all: sidecond_hammer.
+  Unshelve. all: print_remaining_sidecond.
+Qed.
+End proof.
